.

coq/theories/PetitSQL.v
@@ -8,6 +8,106 @@ Require Import Coq.Program.Program.
 Require Import Coq.Strings.Byte.
 Require Import Coq.Strings.String.
 
+Module Utils.
+
+  Lemma lt_strongInd (P : nat -> Prop)
+    (IND : forall n : nat, forall IH : forall m : nat, m < n -> P m, P n)
+    : forall n : nat, P n.
+  Proof.
+    intros n. eapply IND. induction n as [ | n IH].
+    - intros m H_lt. inversion H_lt.
+    - intros m H_lt. eapply IND.
+      intros i i_lt_m. eapply IH. lia.
+  Defined.
+
+  Lemma acc_lt
+    : forall x : nat, Acc Nat.lt x.
+  Proof. exact (lt_strongInd (@Acc nat Nat.lt) (@Acc_intro nat Nat.lt)). Defined.
+
+  Lemma acc_rel {A : Type} {B : Type} (f : A -> B) (R : B -> B -> Prop)
+    (R_wf : forall y : B, Acc R y)
+    : forall x : A, Acc (fun lhs : A => fun rhs : A => R (f lhs) (f rhs)) x.
+  Proof.
+    intros x. remember (f x) as y eqn: y_eq_f_x.
+    revert x y_eq_f_x. induction (R_wf y) as [y' hyp_wf IH].
+    intros x' hyp_eq. econstructor. intros x f_x_R_f_x'.
+    subst y'. eapply IH; [exact (f_x_R_f_x') | reflexivity].
+  Defined.
+
+End Utils.
+
+Export Utils.
+
+Module P.
+
+  Import ListNotations.
+
+  Definition parser (A : Type) : Type := string -> option (A * string).
+
+  Definition runParser {A : Type} (p : parser A) (s : string) : option (A * string) := p s.
+
+  Class Monad (M : Type -> Type) : Type :=
+    { pure {A : Type} : A -> M A
+    ; bind {A : Type} {B : Type} : M A -> (A -> M B) -> M B
+    }.
+
+  Global Infix " >>= " := bind (left associativity, at level 90).
+
+  Global Instance parserMonad : Monad parser :=
+    { pure {A} := fun x : A => fun s : string => Some (x, s)
+    ; bind {A} {B} := fun m : parser A => fun k : A -> parser B => fun s : string =>
+      match m s with
+      | None => None
+      | Some (x, s') => k x s'
+      end
+    }.
+
+  Definition empty {A : Type} : parser A :=
+    fun s : string => None.
+
+  Definition alt {A : Type} (p1 : parser A) (p2 : parser A) : parser A := fun s : string =>
+    match p1 s with
+    | None => p2 s
+    | Some (x, s') => Some (x, s')
+    end.
+
+  Global Infix " <|> " := alt (left associativity, at level 50).
+
+  Definition isLt {A : Type} (p : parser A) : Prop :=
+    forall s : string,
+    match p s with
+    | None => True
+    | Some (x, s') => length s' < length s
+    end.
+
+  Definition isLe {A : Type} (p : parser A) : Prop :=
+    forall s : string,
+    match p s with
+    | None => True
+    | Some (x, s') => length s' <= length s
+    end.
+
+  Definition some {A : Type}
+    (p1 : parser A)
+    (p1_isLt : isLt p1)
+    : {p : parser (list A) | isLe p}.
+  Proof.
+    enough (TO_SHOW : forall s : string, {ret : option (list A * string) | match ret with None => True | Some (x, s') => length s' <= length s end}).
+    { exact (@exist (parser (list A)) isLe (fun s => proj1_sig (TO_SHOW s)) (fun s => proj2_sig (TO_SHOW s))). }
+    enough (MAIN : forall s : string, Acc (fun s1 : string => fun s2 : string => length s1 < length s2) s -> {ret : option (list A * string) | match ret with None => True | Some (x, s') => length s' <= length s end}).
+    { intros s. exact (MAIN s (Utils.acc_rel length Nat.lt acc_lt s)). }
+    apply (@Acc_rect string (fun s1 : string => fun s2 : string => length s1 < length s2) (fun s : string => {ret : option (list A * string) | match ret with None => True | Some (x, s') => length s' <= length s end})).
+    intros s _ IH. destruct (p1 s) as [[x s'] | ] eqn: H_p1_s.
+    - pose proof (p1_isLt s) as s_isLongerThan_s'.
+      rewrite H_p1_s in s_isLongerThan_s'.
+      destruct (IH s' s_isLongerThan_s') as [[[xs s''] | ] H_ps] eqn: H_ps_s'.
+      + exists (Some ((x :: xs), s'')). lia.
+      + exists (Some ([], s')). lia.
+    - exists (None). trivial.
+  Defined.
+
+End P.
+
 Module Hs.
 
   Inductive strSQLElem : Set :=
